src/Extraction.v
@@ -1,9 +1,9 @@
 (* need this or the Haskell extraction fails *)
 Set Printing Width 1300000.
 
-Require Import Coq.Lists.List.
 Require Import Coq.Strings.Ascii.
 Require Import Coq.Strings.String.
+Require Import Coq.Lists.List.
 
 Require Import Preamble.
 Require Import General.
@@ -25,7 +25,7 @@ Require Import HaskProof.
 Require Import HaskCoreToWeak.
 Require Import HaskWeakToStrong.
 Require Import HaskStrongToProof.
-(*Require Import HaskProofToStrong.*)
+Require Import HaskProofToStrong.
 Require Import HaskProofToLatex.
 Require Import HaskStrongToWeak.
 Require Import HaskWeakToCore.
@@ -33,13 +33,14 @@ Require Import HaskWeakToCore.
 Open Scope string_scope.
 Extraction Language Haskell.
 
+(*Extract Inductive vec    => "([])" [ "([])" "(:)" ].*)
+(*Extract Inductive Tree   => "([])" [ "([])" "(:)" ].*)
+(*Extract Inlined Constant map => "Prelude.map".*)
+
 (* I try to reuse Haskell types mostly to get the "deriving Show" aspect *)
 Extract Inductive option => "Prelude.Maybe" [ "Prelude.Just" "Prelude.Nothing" ].
 Extract Inductive list   => "([])" [ "([])" "(:)" ].
-(*Extract Inductive vec    => "([])" [ "([])" "(:)" ].*)
-(*Extract Inductive Tree   => "([])" [ "([])" "(:)" ].*)
-Extract Inlined Constant map => "Prelude.map".
-Extract Inductive string => "Prelude.String" [ "([])" "(:)" ].
+Extract Inductive string => "Prelude.String" [ "[]" "(:)" ].
 Extract Inductive prod   => "(,)" [ "(,)" ].
 Extract Inductive sum    => "Prelude.Either" [ "Prelude.Left" "Prelude.Right" ].
 Extract Inductive sumbool => "Prelude.Bool" [ "Prelude.True" "Prelude.False" ].
@@ -47,10 +48,9 @@ Extract Inductive bool    => "Prelude.Bool" [ "Prelude.True" "Prelude.False" ].
 Extract Inductive unit    => "()" [ "()" ].
 Extract Inlined Constant string_dec => "(==)".
 Extract Inlined Constant ascii_dec => "(==)".
-Extract Inductive string => "Prelude.String" [ "[]" "(:)" ].
 
 (* adapted from ExtrOcamlString.v *)
-Extract Inductive ascii => "Prelude.Char" [ "bin2ascii" ] "bin2ascii'".
+Extract Inductive ascii => "Char" [ "bin2ascii" ] "bin2ascii'".
 Extract Constant zero   => "'\000'".
 Extract Constant one    => "'\001'".
 Extract Constant shift  => "shiftAscii".
@@ -58,10 +58,10 @@ Extract Constant shift  => "shiftAscii".
 Unset Extraction Optimize.
 Unset Extraction AutoInline.
 
-
 Variable Name : Type.  Extract Inlined Constant Name => "Name.Name".
 Variable mkSystemName : Unique -> string -> nat -> Name.
-  Extract Inlined Constant mkSystemName => "(\u s d -> Name.mkSystemName u (OccName.mkOccName (OccName.varNameDepth (nat2int d)) s))".
+  Extract Inlined Constant mkSystemName =>
+    "(\u s d -> Name.mkSystemName u (OccName.mkOccName (OccName.varNameDepth (nat2int d)) s))".
 Variable mkTyVar : Name -> Kind -> CoreVar.
   Extract Inlined Constant mkTyVar => "(\n k -> Var.mkTyVar n (kindToCoreKind k))".
 Variable mkCoVar : Name -> CoreType -> CoreType -> CoreVar.
@@ -116,6 +116,7 @@ Section core2proof.
     eol+++"\end{document}"+++
     eol.
 
+
   Definition coreToStringExpr' (ce:@CoreExpr CoreVar) : ???string :=
     addErrorMessage ("input CoreSyn: " +++ ce)
     (addErrorMessage ("input CoreType: " +++ coreTypeOfCoreExpr ce) (
@@ -162,6 +163,124 @@ Section core2proof.
     Context (hetmet_esc   : WeakExprVar).
     Context (uniqueSupply : UniqSupply).
 
+    Definition useUniqueSupply {T}(ut:UniqM T) : ???T :=
+      match ut with
+        uniqM f =>
+         f uniqueSupply >>= fun x => OK (snd x)
+      end.
+
+    Definition larger : forall ln:list nat, { n:nat & forall n', In n' ln -> gt n n' }.
+      intros.
+      induction ln.
+      exists O.
+      intros.
+      inversion H.
+      destruct IHln as [n pf].
+      exists (plus (S n) a).
+      intros.
+      destruct H.
+      omega.
+      fold (@In _ n' ln) in H.
+      set (pf n' H) as q.
+      omega.
+      Defined.
+ 
+  Definition FreshNat : @FreshMonad nat.
+    refine {| FMT       := fun T => nat -> prod nat T
+            ; FMT_fresh := _
+           |}.
+    Focus 2.
+    intros.
+    refine ((S H),_).
+    set (larger tl) as q.
+    destruct q as [n' pf].
+    exists n'.
+    intros.
+    set (pf _ H0) as qq.
+    omega.
+    
+    refine {| returnM := fun a (v:a) => _ |}.
+      intro n. exact (n,v).
+      intros.
+      set (X H) as q.
+      destruct q as [n' v].
+      set (X0 v n') as q'.
+      exact q'.
+      Defined.
+
+    Definition unFresh {T} : @FreshM _ FreshNat T -> T.
+      intros.
+      destruct X.
+      exact O.
+      apply t.
+      Defined.
+
+    Definition env := ★::nil.
+    Definition freshTV : HaskType env ★ := haskTyVarToType (FreshHaskTyVar _).
+    Definition idproof0 : ND Rule [] [env > nil > [] |- [freshTV--->freshTV @@ nil]].
+      eapply nd_comp.
+      eapply nd_comp.
+      eapply nd_rule.
+      apply RVar.
+      eapply nd_rule.
+      eapply (RURule _ _ _ _ (RuCanL _ _)) .
+      eapply nd_rule.
+      eapply RLam.
+      Defined.
+(*
+    Definition TInt : HaskType nil ★.
+      assert (tyConKind' intPrimTyCon = ★).
+        admit.
+        rewrite <- H.
+        unfold HaskType; intros.
+        apply TCon.
+        Defined.
+
+    Definition idproof1 : ND Rule [] [nil > nil > [TInt @@ nil] |- [TInt @@ nil]].
+      apply nd_rule.
+      apply RVar.
+      Defined.
+
+    Definition idtype :=
+        HaskTAll(Γ:=nil) ★ (fun TV ite tv => (TApp (TApp TArrow (TVar tv)) (TVar tv))).
+
+    Definition idproof : ND Rule [] [nil > nil > [] |- [idtype @@ nil]].
+      eapply nd_comp; [ idtac | eapply nd_rule ; eapply RAbsT ].
+      apply idproof0.
+      Defined.
+*)
+(*
+    Definition coreToCoreExpr' (ce:@CoreExpr CoreVar) : ???(@CoreExpr CoreVar) :=
+    addErrorMessage ("input CoreSyn: " +++ ce)
+    (addErrorMessage ("input CoreType: " +++ coreTypeOfCoreExpr ce) (
+      coreExprToWeakExpr ce >>= fun we =>
+        addErrorMessage ("WeakExpr: " +++ we)
+          ((addErrorMessage ("CoreType of WeakExpr: " +++ coreTypeOfCoreExpr (weakExprToCoreExpr we))
+            ((weakTypeOfWeakExpr we) >>= fun t =>
+              (addErrorMessage ("WeakType: " +++ t)
+                ((weakTypeToTypeOfKind φ t ★) >>= fun τ =>
+                  addErrorMessage ("HaskType: " +++ τ)
+                  ((weakExprToStrongExpr Γ Δ φ ψ ξ (fun _ => true) τ nil we) >>= fun e =>
+                        (let haskProof := @expr2proof _ _ _ _ _ _ e
+                          in (* insert HaskProof-to-HaskProof manipulations here *)
+                   (unFresh (@proof2expr nat _ FreshNat _ _ _ _ (fun _ => Prelude_error "unbound unique") _ haskProof))
+                  >>= fun e' => Error (@toString _ (ExprToString _ _ _ _) (projT2 e'))
+(*
+                  >>= fun e' =>
+                    Prelude_error (@toString _ (@ExprToString nat _ _ _ _ _ _) (projT2 e'))
+  *)                  
+)
+)))))))).
+(*                    Error "X").*)
+(*
+                   strongExprToWeakExpr hetmet_brak hetmet_esc mkWeakTypeVar mkWeakCoerVar mkWeakExprVar uniqueSupply
+                   (projT2 e')
+                         INil
+                         >>= fun q => Error (toString q)
+                  ))))))))).
+*)
+*)
+
     Definition coreToCoreExpr' (ce:@CoreExpr CoreVar) : ???(@CoreExpr CoreVar) :=
       addErrorMessage ("input CoreSyn: " +++ ce)
       (addErrorMessage ("input CoreType: " +++ coreTypeOfCoreExpr ce) (
@@ -173,13 +292,18 @@ Section core2proof.
                   ((weakTypeToTypeOfKind φ t ★) >>= fun τ =>
 
                     ((weakExprToStrongExpr Γ Δ φ ψ ξ (fun _ => true) τ nil we) >>= fun e =>
-                      (* insert HaskStrong-to-HaskStrong manipulations here *)
-                      strongExprToWeakExpr hetmet_brak hetmet_esc mkWeakTypeVar mkWeakCoerVar mkWeakExprVar uniqueSupply e INil
-                      >>= fun q => OK (weakExprToCoreExpr q)
-(*
-                    OK (weakExprToCoreExpr we)
-*)
-                    )))))))).
+
+                      (addErrorMessage ("HaskStrong...")
+                        (let haskProof := @expr2proof _ _ _ _ _ _ e
+                         in (* insert HaskProof-to-HaskProof manipulations here *)
+                         OK ((@proof2expr nat _ FreshNat _ _ _ _ (fun _ => Prelude_error "unbound unique") _ haskProof) O)
+                         >>= fun e' =>
+                           (snd e') >>= fun e'' =>
+                         strongExprToWeakExpr hetmet_brak hetmet_esc mkWeakTypeVar mkWeakCoerVar mkWeakExprVar uniqueSupply
+                           (projT2 e'') INil
+                         >>= fun q =>
+                           OK (weakExprToCoreExpr q)
+                    )))))))))).
 
     Definition coreToCoreExpr (ce:@CoreExpr CoreVar) : (@CoreExpr CoreVar) :=
       match coreToCoreExpr' ce with
@@ -212,6 +336,7 @@ Section core2proof.
     end.
 
 End core2proof.
-
+(*Set Extraction Optimize.*)
+(*Set Extraction AutoInline.*)
 Extraction "Extraction.hs" coqPassCoreToString coqPassCoreToCore.
 
